Proofs/one_equals_one.v
@@ -2,23 +2,36 @@ Require Import Vloc.Lib.theory.
 
 Require Import Vloc.CCode.ret_one.
 
-Instance CompSpecs : compspecs. make_compspecs prog. Defined.
+#[local] Instance CompSpecs : compspecs. make_compspecs prog. Defined.
 Definition Vprog : varspecs.  mk_varspecs prog. Defined.
 
+#[local] Instance one_ctx : refines_ctx := { gName := 1; nspace := nroot .@ "test"}.
+
+Definition refines f2 A : funspec :=
+  WITH gv: globals, ctx: ref_id
+  PRE [ (* types of function parameters *) ]
+    PROP()
+    PARAMS((* NOTE: how to handle parameters *))
+    GLOBALS((* do we need anything to correlate globals and Context? Hopefully not *))
+    SEP(refines_right ctx f2)
+  POST [ tint ] (* NOTE: type!!! A map of iris types to vst types? *)
+    EX v' : ival, EX v : val,
+    PROP()
+    RETURN(v)
+    SEP(refines_right ctx (ectxi_language.of_val v') * A v v').
 
 
 (* I shouldn't have to do this, I think *)
-Definition refines_heap_lang e A : funspec := refines  (gName := theory.gName) (nspace:= theory.nspace) e A.
 
 Definition ret_one : iexp := Val (LitV (heap_lang.LitInt 1%Z)).
 (*NOTE: diff between ectxi language and ectx language?*)
-Definition fspec := DECLARE _returns_one refines_heap_lang ret_one 
+Definition fspec := DECLARE _returns_one refines ret_one 
   (fun vVST vHL => !! (exists n : Z, vVST = Vint (Int.repr n) /\ vHL = LitV (heap_lang.LitInt n%Z))&&emp)%logic.
 Definition Gprog : funspecs := [fspec].
 
 Lemma one: semax_body Vprog Gprog f_returns_one fspec.
 Proof.
-  unfold fspec, refines_heap_lang, refines.
+  unfold fspec, refines, refines.
   start_function.
   forward.
   Exists (LitV (heap_lang.LitInt 1%Z)).
@@ -32,12 +45,11 @@ Qed.
 
 Definition ret_one_plus : iexp := BinOp PlusOp (Val (LitV (heap_lang.LitInt 1%Z))) (Val (LitV (heap_lang.LitInt 0%Z))).
 
-Lemma one_plus_zero : semax_body Vprog Gprog f_returns_one (DECLARE _returns_one refines_heap_lang ret_one_plus
+Lemma one_plus_zero : semax_body Vprog Gprog f_returns_one (DECLARE _returns_one refines ret_one_plus
   (fun vVST vHL => !! (exists n : Z, vVST = Vint (Int.repr n) /\ vHL = LitV (heap_lang.LitInt n%Z)) && emp)%logic).
 Proof.
-  unfold fspec, refines_heap_lang, refines.
+  unfold fspec, refines, refines.
   start_function.
-  unfold ret_one_plus.
   step_pure_r ctx.
   forward.
   Exists (LitV (heap_lang.LitInt 1%Z)).
@@ -47,17 +59,27 @@ Proof.
 Qed.
 
 Definition ret_one_min_plus : iexp := BinOp PlusOp 
-  (BinOp MinusOp (Val (LitV (heap_lang.LitInt 1%Z)))  (Val (LitV (heap_lang.LitInt 1%Z))))
-  (Val (LitV (heap_lang.LitInt 0%Z))).
+  (BinOp MinusOp (Val (LitV (heap_lang.LitInt 1%Z)))  (Val (LitV (heap_lang.LitInt (-1)%Z))))
+  (Val (LitV (heap_lang.LitInt (-1)%Z))).
 
-Lemma one_plus_zero' : semax_body Vprog Gprog f_returns_one (DECLARE _returns_one refines_heap_lang ret_one_min_plus
+Lemma one_plus_zero' : semax_body Vprog Gprog f_returns_one (DECLARE _returns_one refines ret_one_min_plus
   (fun vVST vHL => !! (exists n : Z, vVST = Vint (Int.repr n) /\ vHL = LitV (heap_lang.LitInt n%Z)) && emp)%logic).
 Proof.
-  unfold fspec, refines_heap_lang, refines.
+  unfold fspec, refines, refines.
   start_function.
   Fail step_pure_r ctx.
+  unfold ret_one_min_plus.
+  step_pure_r ctx.
+  step_pure_r ctx.
   forward.
-  Exists (LitV (heap_lang.LitInt 1%Z)).
-  Exists (Vint (Int.repr 1)).
-  entailer!; eauto.
-Admitted.
+
+  (* fun with seeing evars to see if this is nicer *)
+  evar (a : ival).
+  Exists a.
+  evar (b : val).
+  Exists b.
+  entailer!.
+  - split; eauto.
+    subst b; auto.
+  - subst a; apply derives_refl.
+Qed.
