Proofs/fact.v
@@ -14,9 +14,9 @@ End iris.
 Require Import Vloc.Lib.theory.
 Require Import Vloc.CCode.fact.
 
-Instance fact_ctx : refines_ctx := { gName := 1; nspace := nroot .@ "test"}.
+#[local] Instance fact_ctx : refines_ctx := { gName := 1; nspace := nroot .@ "test"}.
 
-Instance CompSpecs : compspecs. make_compspecs prog. Defined.
+#[local] Instance CompSpecs : compspecs. make_compspecs prog. Defined.
 Definition Vprog : varspecs.  mk_varspecs prog. Defined.
 
 (* here, the refines we had before won't work... *)
@@ -46,62 +46,7 @@ Ltac print_goal := match goal with
 Lemma one_plus_zero : semax_body Vprog Gprog f_factorial fspec.
 Proof.
   start_function. 
-  unfold iris.factI.
-  forward.
-
-  (*evar (thing : iexp).*)
-  (*assert ((PureExec True  1*)
-   (*(heap_lang.Rec "factI" "n"*)
-      (*(If (BinOp EqOp (Var "n") (Val (LitV (LitInt 0))))*)
-         (*(Val (LitV (LitInt 1)))*)
-         (*(BinOp MultOp (Var "factI")*)
-            (*(BinOp MinusOp (Var "n") (Val (LitV (LitInt 1))))))) thing)).*)
-            (*{*)
-              (*eapply (pure_recc _).*)
-            (*}*)
-
-  match goal with
-  | |- context[refines_right ctx ?expr] => 
-      reshape_expr expr ltac:(fun K e => 
-        replace expr with (fill K e) by (by rewrite ? fill_app);
-        evar (e' : iexp);
-        viewshift_SEP 0 (refines_right ctx (fill K e'));
-        first (
-          go_lower; 
-          eapply (refines_right_pure_r e e' _ _ _ K 1);
-          [try_pures | auto | auto]
-        );
-        simpl in e';
-        subst e'
-        )
-  end.
-  evar (e' : iexp);
-  match goal with
-  | |- context[refines_right ctx expr] =>
-      replace expr with () 
-  end.
-
-
-
-        go_lower; eapply (refines_right_pure_r _ _ _ _ _ K' 1) ) end.
-        [ try_pures | auto | auto ]; simpl in e''; subst e''
-     )
-  end.
-  eapply (refines_right_pure_r _ _ _ _ _ [] 1); [| auto | auto].
-  eapply (pure_exec_ctx (Λ := heap_lang) _ [Val (RecV "FactI" "n" _)]).
-
   step_pure_r ctx.
-  unfold refines_right.
-  unfold spec_ctx.
-  unfold spec_inv.
-
-  evar (e' : iexp).
-  viewshift_SEP 0 (@refines_right theory.gName theory.nspace ctx e').
-  go_lower.
-  eapply (refines_right_pure_r _ _ _ _ _ [] 1); [| auto | auto].
-  eapply (pure_exec_ctx (Λ := heap_lang) _ [Val (RecV "FactI" "n" _)]).
-
-
-
-  forward_loop (acc).
-  
+  forward.
+  step_pure_r ctx.
+Admitted.
